lean/WarpTypes.lean
@@ -1,5 +1,6 @@
 -- This module serves as the root of the `WarpTypes` library.
 -- Import modules here that should be built as part of the library.
+import WarpTypes.Generic
 import WarpTypes.Basic
 import WarpTypes.Metatheory
 import WarpTypes.SolExperiment
